Bench.v
@@ -27,5 +27,18 @@ Definition fSSNI_smart := propSSNI_smart exp_result_fuzz.
 Definition rSSNI_naive := propSSNI_arb   exp_result_random.
 Definition fSSNI_naive := propSSNI_arb   exp_result_fuzz.
 
+Definition nth_table n := nth n (mutate_table default_table) default_table.
+
+Definition qcfSSNI_copy_prop_0 :=
+  fun v => propSSNI_helper (nth_table 0) v exp_result_opt_bool.
+
+Definition qcfSSNI_copy_loop_0 :=
+  fuzzLoop gen_variation_copy fuzz show qcfSSNI_copy_prop_0.
+
+ManualExtract [BinOpT; Label; Instr; Pointer; Value; Atom; Ptr_atom; StackFrame; Stack; memframe; State; Variation].
+
+FuzzQC qcfSSNI_copy_prop_0 qcfSSNI_copy_loop_0.
+(*
 QuickChick (testMutantX_ rSSNI_naive 0).
 FuzzChick (testMutantX_ 0).
+*)
